Theorems.v
@@ -361,3 +361,275 @@ Section CombineActionsTraceInclusion.
     econstructor; eauto.
   Qed.
 End CombineActionsTraceInclusion.
+
+Section InversionSemActionTree.
+  Variable t: Tree ModStateElem.
+
+  Theorem InversionSemActionTree
+    k (a: @ActionTree type t k) old new ret
+    (semA: SemActionTree a old new ret):
+    match a with
+    | ReadRegTree s x cont => SemActionTree (cont (castStateReg x (readTreeState t old x.(regPath)))) old new ret
+    | WriteRegTree x v cont =>
+        SemActionTree cont (writeTreeState t old x.(regPath) (castStateRegInv x (evalExpr v))) new ret
+    | ReadRqMemTree x i p cont =>
+        SemActionTree
+          cont
+          (let arr := castStateMem x (readTreeState t old x.(memPath)) in
+           let val := readNatToFinType (Default _) (readSameTuple (fst arr)) (Z.to_nat (Zmod.to_Z (evalExpr i))) in
+           writeTreeState t old x.(memPath) (castStateMemInv x (fst arr, updSameTuple (snd arr) p val))) new ret
+    | ReadRpMemTree s x p cont =>
+        SemActionTree (cont (readSameTuple (snd (castStateMem x (readTreeState t old x.(memPath)))) p)) old new ret
+    | WriteMemTree x i v cont =>
+        SemActionTree
+          cont
+          (let arr := castStateMem x (readTreeState t old x.(memPath)) in
+           writeTreeState t old x.(memPath) (castStateMemInv x (updSameTupleNat (fst arr) (Z.to_nat (Zmod.to_Z (evalExpr i))) (evalExpr v), snd arr))) new ret
+    | SendTree x v cont =>
+        SemActionTree cont
+          (let currentTrace := castStateSend x (readTreeState t old x.(sendPath)) in
+           writeTreeState t old x.(sendPath) (castStateSendInv x (evalExpr v :: currentTrace)))
+          new ret
+    | RecvTree s x cont =>
+        exists recvVal,
+        SemActionTree (cont recvVal)
+          (let currentTrace := castStateRecv x (readTreeState t old x.(recvPath)) in
+           writeTreeState t old x.(recvPath) (castStateRecvInv x (recvVal :: currentTrace)))
+          new ret
+    | LetExpTree s k' e cont =>
+        SemActionTree (cont (evalExpr e)) old new ret
+    | LetActionTree s k' a' cont =>
+        exists newStep retStep,
+        SemActionTree a' old newStep retStep /\
+          SemActionTree (cont retStep) newStep new ret
+    | NonDetTree s k' cont =>
+        exists v,
+        SemActionTree (cont v) old new ret
+    | IfElseTree s p k' t_branch f_branch cont =>
+        exists newStep retStep,
+        (evalExpr p = true -> SemActionTree t_branch old newStep retStep) /\
+          (evalExpr p = false -> SemActionTree f_branch old newStep retStep) /\
+          SemActionTree (cont retStep) newStep new ret
+    | SystemTree ls cont =>
+        SemActionTree cont old new ret
+    | ReturnTree e =>
+        new = old /\ ret = evalExpr e
+    end.
+  Proof.
+    destruct semA; eauto; repeat eexists; eauto; try discriminate.
+  Qed.
+End InversionSemActionTree.
+
+Definition InitStateElemConsistentPf (e: ModStateElem) : InitStateElemConsistent e (InitStateElem e) :=
+  match e return InitStateElemConsistent e (InitStateElem e) with
+  | ERegister r =>
+      match r.(registerInit) as opt return
+        (match opt with
+         | None => fun s => True
+         | Some init => fun s => s = init
+         end)
+        (match opt with
+         | None => Default (registerKind r)
+         | Some init => init
+         end)
+      with
+      | None => I
+      | Some init => eq_refl
+      end
+  | EMemory m =>
+      match m.(memoryInit) as opt return
+        (match opt with
+         | None => fun s => True
+         | Some _ => fun s => fst s = memoryInitFull m
+         end) (memoryInitFull m, Default (Array m.(memoryPort) m.(memoryKind)))
+      with
+      | None => I
+      | Some _ => eq_refl
+      end
+  | ESend _ => eq_refl
+  | ERecv _ => eq_refl
+  end.
+
+Fixpoint InitStateConsistentPf (t: Tree ModStateElem) : InitStateConsistent t (InitState t) :=
+  match t return InitStateConsistent t (InitState t) with
+  | Leaf name a => InitStateElemConsistentPf a
+  | Node name children =>
+      (fix loop (ls: list (Tree ModStateElem)) :
+         (fix loop (ls : list (Tree ModStateElem)) : ModListTreeState ls -> Prop :=
+            match ls with
+            | nil => fun _ => True
+            | x :: xs => fun s => InitStateConsistent x (fst s) /\ loop xs (snd s)
+            end) ls
+           ((fix loop (ls : list (Tree ModStateElem)) : ModListTreeState ls :=
+              match ls with
+              | nil => tt
+              | x :: xs => (InitState x, loop xs)
+              end) ls) :=
+         match ls return
+           (fix loop (ls : list (Tree ModStateElem)) : ModListTreeState ls -> Prop :=
+              match ls with
+              | nil => fun _ => True
+              | x :: xs => fun s => InitStateConsistent x (fst s) /\ loop xs (snd s)
+              end) ls
+             ((fix loop (ls : list (Tree ModStateElem)) : ModListTreeState ls :=
+                match ls with
+                | nil => tt
+                | x :: xs => (InitState x, loop xs)
+                end) ls)
+         with
+         | nil => I
+         | x :: xs => conj (InitStateConsistentPf x) (loop xs)
+         end) children
+  end.
+
+Definition ExistsInitModConsistentTree (t: Tree ModStateElem) : exists old, InitStateConsistent t old.
+Proof.
+  exists (InitState t).
+  apply InitStateConsistentPf.
+Qed.
+
+Section StepInclusionTree.
+  Variable t1 t2: Tree ModStateElem.
+  Variable m1: ModTree t1.
+  Variable m2: ModTree t2.
+  Variable rel: ModTreeState t1 -> ModTreeState t2 -> Prop.
+  Variable relConsistent: forall old1 old2,
+      InitStateConsistent t1 old1 ->
+      rel old1 old2 ->
+      InitStateConsistent t2 old2.
+
+  Variable stepMod: forall a1 old1 new1,
+      In a1 (m1 type) ->
+      SemActionTree a1 old1 new1 Zmod.zero ->
+      forall old2: ModTreeState t2,
+        rel old1 old2 ->
+        exists a2 new2,
+          In a2 (m2 type) /\ rel new1 new2 /\
+          SemActionTree a2 old2 new2 Zmod.zero.
+
+  Lemma stepInclusionHelperTree: forall s1 s2,
+      SemAnyActionTree (m1 type) s1 s2 ->
+      forall old2,
+        rel s1 old2 ->
+        exists new2,
+          rel s2 new2 /\
+          SemAnyActionTree (m2 type) old2 new2.
+  Proof.
+    induction 1 as [old_nil new_nil eqPf | old_cons new_cons newStep step rest IHrest]; intros.
+    - subst.
+      exists old2.
+      split; [exact H | constructor 1; auto].
+    - destruct step.
+      specialize (@stepMod a old newStep inA aPf old2 H) as H_step.
+      destruct H_step as [a2 [newStep2 [inA2 [relNewStep2 semA2]]]].
+      specialize (IHrest newStep2 relNewStep2) as [new2 [relNew2 restSteps]].
+      exists new2.
+      split; [exact relNew2 |].
+      econstructor 2; eauto.
+      constructor 1 with (a := a2); auto.
+  Qed.
+
+  Theorem StepInclusionTree: TraceInclusionTree m1 m2 rel.
+  Proof.
+    intros old1 new1 H_sem old2 relOld.
+    destruct H_sem as [old1 new1 old1Consistent semAny1].
+    pose proof (@relConsistent old1 old2 old1Consistent relOld) as old2Consistent.
+    pose proof (stepInclusionHelperTree semAny1 relOld) as [new2 [relNew2 semAny2]].
+    exists new2.
+    split.
+    - constructor; auto.
+    - exact relNew2.
+  Qed.
+End StepInclusionTree.
+
+Section CombineActionsTreeHelpers.
+  Variable t: Tree ModStateElem.
+
+  Lemma addStepTree ls old new:
+    StepTree ls old new ->
+    forall (act: @ActionTree type t (Bit 0)),
+      StepTree (act :: ls) old new.
+  Proof.
+    intros.
+    destruct H; subst.
+    constructor 1 with (a := a); simpl; tauto.
+  Qed.
+
+  Lemma addSemAnyActionTree ls old new:
+    SemAnyActionTree ls old new ->
+    forall (a: @ActionTree type t (Bit 0)),
+      SemAnyActionTree (a :: ls) old new.
+  Proof.
+    induction 1; subst; intros.
+    - constructor 1; auto.
+    - econstructor 2 with (newStep := newStep); eauto.
+      apply addStepTree; auto.
+  Qed.
+
+  Lemma combineSemActionToSemAnyActionTree (ls: list (@ActionTree type t (Bit 0))):
+    forall old new,
+      SemActionTree (combineActionsTree ls) old new Zmod.zero ->
+      SemAnyActionTree ls old new.
+  Proof.
+    induction ls; simpl; intros; apply InversionSemActionTree in H; cbn in H.
+    - destruct H; subst.
+      constructor 1; auto.
+    - destruct H as [newStep [retStep [semA semCb]]].
+      specialize (IHls _ _ semCb).
+      pose proof (Zmod.hprop_Zmod_1 retStep Zmod.zero) as retEq.
+      subst.
+      pose proof (addSemAnyActionTree IHls a) as pf.
+      econstructor 2 with (newStep := newStep); eauto.
+      econstructor; eauto.
+      simpl; tauto.
+  Qed.
+
+  Section CombineSemAnyActionTree.
+    Variable ls: list (@ActionTree type t (Bit 0)).
+    Lemma combineSemAnyActionsTree:
+      forall old new1 new2,
+        SemAnyActionTree ls old new1 ->
+        SemAnyActionTree ls new1 new2 ->
+        SemAnyActionTree ls old new2.
+    Proof.
+      induction 1 as [old_nil new_nil eqPf | old_cons new_cons newStep step rest IHrest]; intros.
+      - subst.
+        exact H.
+      - econstructor 2 with (newStep := newStep); eauto.
+    Qed.
+  End CombineSemAnyActionTree.
+
+  Lemma combineActionsSemanticsTree (ls: list (@ActionTree type t (Bit 0))):
+    forall old new,
+      SemAnyActionTree (combineActionsTree ls :: nil) old new ->
+      SemAnyActionTree ls old new.
+  Proof.
+    induction 1 as [old_nil new_nil eqPf | old_cons new_cons newStep step rest IHrest]; intros.
+    - constructor 1; subst; auto.
+    - subst.
+      destruct step.
+      destruct inA; [subst | contradiction].
+      apply combineSemActionToSemAnyActionTree in aPf.
+      eapply combineSemAnyActionsTree; eauto.
+  Qed.
+End CombineActionsTreeHelpers.
+
+Section CombineActionsTreeTraceInclusion.
+  Variable t: Tree ModStateElem.
+  Variable ls: forall ty, list (@ActionTree ty t (Bit 0)).
+
+  Theorem CombineActionsTreeTraceInclusion: TraceInclusionTree (fun ty => combineActionsTree (ls ty) :: nil)
+                                                              ls
+                                                              (fun s1 s2 => s1 = s2).
+  Proof.
+    intros old1 new1 H_sem old2 relOld.
+    destruct H_sem as [old1 new1 old1Consistent semAny1].
+    subst old2.
+    apply combineActionsSemanticsTree in semAny1.
+    exists new1.
+    split.
+    - constructor; auto.
+    - reflexivity.
+  Qed.
+End CombineActionsTreeTraceInclusion.
+
